- add ph for a_wl_red_rename_var

proof/old_system/ln_utils.v
@@ -55,6 +55,15 @@ Fixpoint ftvar_in_aworklist' (aW_5:aworklist) : vars :=
   | (aworklist_constvar aW X ab) => (ftvar_in_aworklist' aW) \u (ftvar_in_abind ab) \u (singleton X)
   | (aworklist_conswork aW w) => (ftvar_in_aworklist' aW) \u (ftvar_in_work w)
 end.
+
+
+Fixpoint fvar_in_aworklist' (aW_5:aworklist) : vars :=
+  match aW_5 with
+  | aworklist_empty => {}
+  | (aworklist_consvar aW x ab) => (fvar_in_aworklist' aW) \u (singleton x) (* no var in abind *)
+  | (aworklist_constvar aW X ab) => (fvar_in_aworklist' aW) (* no var in abind *)
+  | (aworklist_conswork aW w) => (fvar_in_aworklist' aW) \u (fvar_in_work w)
+end.
   
 
 Ltac gather_atoms ::=
